Prove equivalence preservation of syntax morphisms

coq/ExpMap.v
@@ -45,16 +45,46 @@ Proof.
 Qed.
 
 Section Morphisms.
+
+  (* Inverted *)
+  Inductive exp_morph' (p2 : polynomial) : polynomial -> Type :=
+  | nil_morph : exp_morph' p2 [::]
+  | cons_morph : forall (S : Set) n (idx : S -> nat) p1,
+      (forall (s : S), (nth zterm p2 (idx s)).1) ->
+      (forall (s : S), Vector.t (Fin.t n) (nth zterm p2 (idx s)).2) ->
+      exp_morph' p2 p1 ->
+      exp_morph' p2 [:: (S,n) & p1].
   
-  Variable p1 p2 : polynomial.
-  
-  Definition exp_morph : Type := forall (S : Set), constr p1 S -> constr p2 S.
+  Fixpoint morph_map {p1 p2} (m : exp_morph' p2 p1) : forall (T : Set), constr p1 T -> constr p2 T.
+    refine( match m with
+            | nil_morph => _
+            | cons_morph S' n idx _ sfn nfn _ => _
+            end).
+    - refine (fun T ce => match ce with
+                        | ccon n s v => _
+                        end).
+      case: n s v; simpl. 
+      + exact (fun ep => match ep with end).
+      + exact (fun _ ep => match ep with end).
+    - refine (fun T ce =>  match ce with
+                           | ccon 0 s v =>
+                             ccon (sfn (s : S'))
+                                  (Vector.map (Vector.nth (v : Vector.t T n))
+                                              (nfn (s : S')))
+                           | ccon n.+1 s v => morph_map _ _ e _ (ccon _ _)
+                           end).
+      exact s.
+      exact v.
+  Defined.
+  (*TODO: finish writing out definition ~nicely *)
   
   Section MorphFns.
 
-    Variable m : exp_morph.
+    Variable p1 p2 : polynomial.
     
-    Definition morph_alg : Alg p1 p2 := fun ce => id_alg (m ce).
+    Variable m : exp_morph' p2 p1.
+    
+    Definition morph_alg : Alg p1 p2 := fun ce => id_alg (morph_map m ce).
     
     Definition morph_fn := alg_fn morph_alg.
     
@@ -81,36 +111,122 @@ Section Morphisms.
       case; auto.
     Qed.
 
-    Lemma morph_alg_comm n s v s'
-      : (morph_alg (ccon s v)) [/ s' /]
-        = morph_alg (@ccon _ _ n s (Vector.map (exp_subst^~ s') v)).
-    Proof.
-      unfold morph_alg.
-      unfold id_alg.
-      (*Issue: this is a sort of paramentricity here! (bad)
-        the best thing is probably to do as I did before and construct an initial
-        representation.
-        Allowed operations:
-        - intuitionistic treatment of subterms (dropping, swapping, duplicating)
-        - functions over coefficients
-       *)          
+  End MorphFns.
+  
+  Lemma vector_map_map {A B C : Type} (g : B -> C) (f : A -> B) n (v : Vector.t A n)
+    : Vector.map g (Vector.map f v) = Vector.map (fun e => g (f e)) v.
+  Proof.
+    elim: v; simpl; auto.
+    move => e1 n' v' ->; done.
+  Qed.
+  
+  Lemma vector_map_nth {B C : Type} (g : B -> C) n (v : Vector.t B n) m
+    : Vector.nth (Vector.map g v) m = g (Vector.nth v m).
+  Proof.
+    elim: v m.
+    - top_inversion.
+    - move => e1 n' v' IH m.
+      move: v' IH.
+      refine (match m as m in Fin.t n'.+1 with
+              | Fin.F1 n'' => _
+              | Fin.FS n'' m' => _
+              end).
+      auto.
+      move => v' IH.
       simpl.
-      elim: p1 p2 n s v s'.
+        by rewrite IH.
+  Qed.
+
+  Lemma vec_map_ext {B C : Type} (f g : B -> C) n (v : Vector.t B n)
+    : (forall e, f e = g e) -> Vector.map f v = Vector.map g v.
+  Proof.
+    move => ext.
+    elim: v; first done.
+    move => e1 n' v' IH.
+    simpl.
+    by rewrite ext IH.
+  Qed.
+
+
+  Tactic Notation "intro_to" constr(ty) :=
+    repeat lazymatch goal with
+           | |- ty -> _ => idtac
+           | |- ty _ -> _ => idtac
+           | |- ty _ _-> _ => idtac
+           | |- ty _ _ _ -> _ => idtac
+           | |- _ -> _ => intro
+           end.
+  
+  Ltac top_inversion :=
+    let f := fresh in
+    intro f; inversion f.
+
+  Tactic Notation "intro_to" constr(ty) "and_invert" :=
+    intro_to ty; top_inversion; subst.
+  
+  Ltac inst_hyp H :=
+  lazymatch type of H with
+  | forall  x : ?T, _ =>
+    match goal with
+      H' : T |- _ =>
+      specialize (H H'); inst_hyp H
+    end
+  | ?T -> _ =>
+    match goal with
+      H' : T |- _ =>
+      specialize (H H'); inst_hyp H
+    end
+  | _ => idtac
+  end.
+  
+  Ltac top_swap :=
+    let n1 := fresh in
+    let n2 := fresh in
+    move => n1 n2;
+    move: n2 n1.
+  
+  Lemma morph_alg_comm {p1 p2} (m : exp_morph' p2 p1) n s v s'
+    : (morph_alg m (ccon s v)) [/ s' /]
+      = morph_alg m (@ccon _ _ n s (Vector.map (exp_subst^~ s') v)).
+  Proof.
+    elim: m n s v s'.
+    - case => [|n]; case.
+    - unfold morph_alg.
+      move => S n.
+      intro_to nat.
+      case.
+      + intros; simpl.
+        f_equal.
+        rewrite vector_map_map.
+        apply: vec_map_ext.
+        move => x.
+        by rewrite vector_map_nth.
+      + intros; simpl.
+        repeat match goal with
+               | |- context [id_alg (morph_map ?M ?E)] =>
+                 change (id_alg (morph_map M E)) with (morph_alg M E)
+               end.
+        apply: H.
+  Qed.        
       
-    Lemma morph_sub_comm e s
-      : morph_fn (e[/s/]) = (morph_fn e)[/List.map morph_fn s/].
-    Proof.
+  Lemma morph_sub_comm {p1 p2} (m : exp_morph' p2 p1) e s
+    : morph_fn m (e[/s/]) = (morph_fn m e)[/List.map (morph_fn m) s/].
+  Proof.
       elim: e; simpl; auto.
       - by apply: morph_lookup.
       - intros.
         unfold morph_fn.
         simpl.
-       
-      
-      elim: s; simpl; auto.
-      rewrite !empty_subst_id => //=.
-      move => a l.
-      Admitted.
+        rewrite morph_alg_comm.
+        repeat f_equal.
+        elim: v H;[by simpl|].
+        simpl.
+        intro_to and.
+        case.
+        do 2 unfold morph_fn at 1.
+        by move -> => /H => ->.
+  Qed.
+
     
     (*TODO: reformulate using a def of preservation? *)
     (*NOTE!!! Assuming this is true, and it should be,
@@ -119,51 +235,51 @@ Section Morphisms.
       Suffices to show that wf_transport (source l) x ->wf  (target l) x?
       I.e. every morphism gives rise to an equivalence preserving compiler
      *)
-    Lemma wf_transport
+    Lemma wf_transport {p1 p2} (m : exp_morph' p2 p1)
       : (forall (l : lang p1) c1 c2 t1 t2,
             le_sort l c1 c2 t1 t2 ->
-            le_sort (lang_fn l) (ctx_fn c1) (ctx_fn c2) (morph_fn t1) (morph_fn t2))
+            le_sort (lang_fn m l) (ctx_fn m c1) (ctx_fn m c2) (morph_fn m t1) (morph_fn m t2))
         /\ (forall (l : lang p1) c1 c2 s1 s2 c1' c2',
                le_subst l c1 c2 s1 s2 c1' c2' ->
-               le_subst (lang_fn l)
-                        (ctx_fn c1) (ctx_fn c2)
-                        (List.map morph_fn s1) (List.map morph_fn s2)
-                        (ctx_fn c1') (ctx_fn c2'))
+               le_subst (lang_fn m l)
+                        (ctx_fn m c1) (ctx_fn m c2)
+                        (List.map (morph_fn m) s1) (List.map (morph_fn m) s2)
+                        (ctx_fn m c1') (ctx_fn m c2'))
         /\ (forall (l : lang p1) c1 c2 e1 e2 t1 t2,
                le_term l c1 c2 e1 e2 t1 t2 ->
-               le_term (lang_fn l)
-                       (ctx_fn c1) (ctx_fn c2)
-                       (morph_fn e1) (morph_fn e2)
-                       (morph_fn t1) (morph_fn t2))
+               le_term (lang_fn m l)
+                       (ctx_fn m c1) (ctx_fn m c2)
+                       (morph_fn m e1) (morph_fn m e2)
+                       (morph_fn m t1) (morph_fn m t2))
         /\ (forall (l : lang p1) c1 c2,
                le_ctx l c1 c2 ->
-               le_ctx (lang_fn l) (ctx_fn c1) (ctx_fn c2))
+               le_ctx (lang_fn m l) (ctx_fn m c1) (ctx_fn m c2))
         /\ (forall (l : lang p1) c1 c2 v1 v2,
                le_ctx_var l c1 c2 v1 v2 ->
-               le_ctx_var (lang_fn l)
-                          (ctx_fn c1) (ctx_fn c2)
-                          (ctx_var_map morph_fn v1) (ctx_var_map morph_fn v2))
+               le_ctx_var (lang_fn m l)
+                          (ctx_fn m c1) (ctx_fn m c2)
+                          (ctx_var_map (morph_fn m) v1) (ctx_var_map (morph_fn m) v2))
         /\ (forall (l : lang p1) c t, 
             wf_sort l c t ->
-            wf_sort (lang_fn l) (ctx_fn c) (morph_fn t))
+            wf_sort (lang_fn m l) (ctx_fn m c) (morph_fn m t))
         /\ (forall (l : lang p1) c s c',
                wf_subst l c s c' ->
-               wf_subst (lang_fn l) (ctx_fn c) (List.map morph_fn s) (ctx_fn c'))
+               wf_subst (lang_fn m l) (ctx_fn m c) (List.map (morph_fn m) s) (ctx_fn m c'))
         /\ (forall (l : lang p1) c e t, 
                wf_term l c e t ->
-               wf_term (lang_fn l) (ctx_fn c) (morph_fn e) (morph_fn t))
-        /\ (forall (l : lang p1) c,  wf_ctx l c -> wf_ctx (lang_fn l) (ctx_fn c))
+               wf_term (lang_fn m l) (ctx_fn m c) (morph_fn m e) (morph_fn m t))
+        /\ (forall (l : lang p1) c,  wf_ctx l c -> wf_ctx (lang_fn m l) (ctx_fn m c))
         /\ (forall (l : lang p1) c v,
                wf_ctx_var l c v ->
-               wf_ctx_var (lang_fn l) (ctx_fn c) (ctx_var_map morph_fn v))
-        /\ (forall (l : lang p1) r,  wf_rule l r -> wf_rule (lang_fn l) (rule_map morph_fn r))
-        /\ (forall (l : lang p1),  wf_lang l -> wf_lang (lang_fn l)).
+               wf_ctx_var (lang_fn m l) (ctx_fn m c) (ctx_var_map (morph_fn m) v))
+        /\ (forall (l : lang p1) r,  wf_rule l r -> wf_rule (lang_fn m l) (rule_map (morph_fn m) r))
+        /\ (forall (l : lang p1),  wf_lang l -> wf_lang (lang_fn m l)).
     Proof.
       apply: mono_ind'; simpl; eauto.
       all: try by intros; rewrite !morph_sub_comm; eauto.
       all: try by intros; (*TODO: write, use intro_to tactic *)
-        apply morph_rule_in in H1; simpl in H1;
-        auto.
+        eapply morph_rule_in in H1; simpl in H1;
+          eauto.
       - intros.
         eapply le_subst_term;
           first by auto.
